bug fix in Alu; first version of revoker

Spec.v
@@ -24,49 +24,32 @@ Set Asymmetric Patterns.
 
 Import ListNotations.
 
+#[projections(primitive)]
+Record MemIfc {mem_t: Tree Elem} {ty: Kind -> Type} := {
+  mem_readBits: ty Addr -> Action ty mem_t (Bit DXlen);
+  mem_readTag: ty (Bit (AddrSz - MemSz)) -> Action ty mem_t Bool;
+  mem_readRevBit: ty (Bit (AddrSz + 1)) -> Action ty mem_t Bool;
+  mem_readInst: ty Addr -> Action ty mem_t Inst;
+  mem_writeBits: ty Addr -> ty (Bit DXlen) -> ty (Bit MemSzSz) -> Action ty mem_t (Bit 0);
+  mem_writeTag: ty (Bit (AddrSz - MemSz)) -> ty Bool -> Action ty mem_t (Bit 0)
+}.
+
 Section Spec.
   Variable MemWidth: nat.
-  Definition LgBytesFullCapSz := Eval compute in Z.to_nat LgNumBytesFullCapSz.
-  Variable MemWidthGeLgBytesFullCapSz: MemWidth >= LgBytesFullCapSz.
-  Definition MemByteSz := Nat.pow 2 MemWidth.
-  Definition MemFullCapSz := Nat.pow 2 (MemWidth - LgBytesFullCapSz).
-  Definition binaryLength := Eval compute in (length binary).
-  Definition specInst: type (Array binaryLength (Bit 8)) := Build_SameTuple (tupleElems := binary)
-                                                                (I: Is_true (length binary =? binaryLength)).
-  Definition MemWidthCap : Z := Z.of_nat MemWidth - LgNumBytesFullCapSz.
+  Variable MemWidthGeLgBytesFullCapSz: MemWidth >= Z.to_nat LgNumBytesFullCapSz.
 
   Variable tohostAddr: type Addr.
 
-      Variable regsInit: type (Array NumRegs FullECapWithTag).
+  Variable regsInit: type (Array NumRegs FullECapWithTag).
   Variable scrsInit: type Scrs.
   Variable csrsInit: type Csrs.
   Variable interruptsInit: type Interrupts.
-  Variable revokerEpochInit: type Data.
-  Variable revokerKickInit: type Bool.
-  Variable revokerStartInit: type (Bit MemWidthCap).
-  Variable revokerEndInit: type (Bit MemWidthCap).
-  Variable revokeAddrInit: type (Bit MemWidthCap).
-
-  Variable RevStart: Z.
-  Variable RevByteSz: Z.
-  Variable RevEachBitLgNumBytes: Z.
-  Variable RevEachBitLgNumBytesInMem: (RevEachBitLgNumBytes < Z.of_nat MemWidth)%Z.
-  Variable RevInMem: (RevStart + RevByteSz < Z.of_nat MemByteSz)%Z.
-  Variable HeapStart: Z.
-  Definition HeapEnd := (HeapStart + (RevByteSz * (Z.shiftl 1 RevEachBitLgNumBytes) * 8))%Z.
-  Variable HeapInMem: (HeapEnd < Z.of_nat MemByteSz)%Z.
-  Variable RevokerAddr: Z.
-  Definition RevokerSize: Z := 4.
-  Definition LgRevokerSzBytes: Z := Z.log2_up XlenBytes + Z.log2_up RevokerSize.
-
-  Definition RevStartAddr: type (Bit (AddrSz + 1)) := bits.of_Z _ RevStart.
-  Definition HeapStartAddr: type (Bit (AddrSz + 1)) := bits.of_Z _ HeapStart.
-  Definition HeapEndAddr: type (Bit (AddrSz + 1)) := bits.of_Z _ HeapEnd.
 
   Local Open Scope string_scope.
   Local Open Scope guru_scope.
 
   Variable mem_t: Tree Elem.
+
   Definition specTree : Tree Elem :=
     Node "" [
       Node "mem" [mem_t];
@@ -74,173 +57,122 @@ Section Spec.
       Leaf "csrs" (EReg {| regKind := Csrs; regInit := Some csrsInit |});
       Leaf "scrs" (EReg {| regKind := Scrs; regInit := Some scrsInit |});
       Leaf "interrupts" (EReg {| regKind := Interrupts; regInit := Some interruptsInit |});
-      Leaf "revokerEpoch" (EReg {| regKind := Data; regInit := Some revokerEpochInit |});
-      Leaf "revokerKick" (EReg {| regKind := Bool; regInit := Some revokerKickInit |});
-      Leaf "revokerStart" (EReg {| regKind := Bit MemWidthCap; regInit := Some revokerStartInit |});
-      Leaf "revokerEnd" (EReg {| regKind := Bit MemWidthCap; regInit := Some revokerEndInit |});
-      Leaf "revokeAddr" (EReg {| regKind := Bit MemWidthCap; regInit := Some revokeAddrInit |});
       Leaf "interrupts_in" (ERecv Interrupts)
     ].
 
-  Definition SpecRevokerAccessState := STRUCT_TYPE {
-                                           "revokerEpoch" :: Data;
-                                           "revokerKick" :: Bool;
-                                           "revokerStart" :: Bit MemWidthCap;
-                                           "revokerEnd" :: Bit MemWidthCap }.
+  Definition np_mem: NodePath specTree mem_t := ltac:(solveNodePath specTree ".mem"%string mem_t).
 
-  Definition SpecProcessorState := STRUCT_TYPE {
-                                       "regs" :: Array NumRegs FullECapWithTag;
-                                       "csrs" :: Csrs;
-                                       "scrs" :: Scrs;
-                                       "interrupts" :: Interrupts;
-                                       "revokerAccess" :: SpecRevokerAccessState }.
   Local Close Scope string_scope.
 
   Section Ty.
     Variable ty: Kind -> Type.
 
-    Definition RevokerEpochAddr: Expr ty Addr := $(RevokerAddr + XlenBytes*0).
-    Definition RevokerKickAddr: Expr ty Addr  := $(RevokerAddr + XlenBytes*1).
-    Definition RevokerStartAddr: Expr ty Addr := $(RevokerAddr + XlenBytes*2).
-    Definition RevokerEndAddr: Expr ty Addr   := $(RevokerAddr + XlenBytes*3).
+    Definition updateArrayBySz (m: Z)
+      (shamt: Expr ty (Bit m))
+      (k: Kind)
+      (n: nat)
+      (oldVal newVal: Expr ty (Array n k))
+      : Expr ty (Array n k) :=
+      ArrayBuilder (fun i => ITE (ReadArrayConst (Not (invMask n shamt)) i)
+                               (ReadArrayConst newVal i)
+                               (ReadArrayConst oldVal i)).
 
-    Definition isInHeap (addr: ty (Bit (AddrSz + 1))): Expr ty Bool :=
-      And [Sge #addr (ConstBit HeapStartAddr); Slt #addr (ConstBit HeapEndAddr)].
+    Definition updateBitsByChunkSz (n: nat) (sz: Z) (m: Z)
+      (shamt: Expr ty (Bit m))
+      (oldVal newVal: Expr ty (Bit (NatZ_mul n sz)))
+      : Expr ty (Bit (NatZ_mul n sz)) :=
+      ToBit (updateArrayBySz shamt
+               (FromBit (Array n (Bit sz)) oldVal)
+               (FromBit (Array n (Bit sz)) newVal)).
 
-    Definition revBitNum (addr: ty (Bit (AddrSz + 1))): Expr ty (Bit (AddrSz + 1)) :=
-      Srl (Sub #addr (ConstBit HeapStartAddr)) (ConstBit (bits.of_Z (Z.of_nat MemWidth) RevEachBitLgNumBytes)).
+    Definition updateWordByByteSz := updateBitsByChunkSz (n := Z.to_nat XlenBytes) (sz := 8).
 
-    Definition revBitByteAddr (addr: ty (Bit (AddrSz + 1))): Expr ty (Bit (AddrSz + 1)) :=
-      Srl (revBitNum addr) (ConstBit (bits.of_Z 2 3)).
+    Variable memIfc: @MemIfc mem_t ty.
 
-    Definition revBitByteOffset (addr: ty (Bit (AddrSz + 1))): Expr ty (Bit 3) :=
-      TruncLsb ((AddrSz + 1) - 3) 3 (revBitNum addr).
+    Definition memLoad (memAddr: ty Addr) (memSz: ty (Bit MemSzSz)) (ldUn: ty Bool)
+      : Action ty mem_t FullECapWithTag :=
+      ( Let isCap : Bool <- isAllOnes #memSz;
+        Let memSzBytes : Bit MemSz <- Sll $1 #memSz;
+        LetA readBits: Bit DXlen <- memIfc.(mem_readBits) memAddr;
+        Let readBytes: Array (Z.to_nat DXlenBytes) (Bit 8) <- FromBit _ #readBits;
+        Let readBitsFixed <- ToBit (ITE #ldUn (ArrayZeroExtend #memSzBytes #readBytes)
+                                      (ArraySignExtend #memSzBytes #readBytes));
+        Let fullCap: FullCap <- FromBit FullCap #readBitsFixed;
+        Let ldCap: Cap <- #fullCap`"cap";
+        Let ldVal: Addr <- #fullCap`"addr";
+        LetL ldECap: ECap <- decodeCap ldCap ldVal;
+        Let ldECapFinal: ECap <- ITE #isCap #ldECap ConstDef;
+        Let memTagAddr: Bit (AddrSz - MemSz) <- TruncMsb _ MemSz #memAddr;
 
-    Definition isRevokerAddr (a: ty Addr) (sz: ty (Bit MemSz)) :=
-      And [Sge #a RevokerEpochAddr; Slt #a RevokerEndAddr; Eq #sz $XlenBytes ].
+        LetA ldTag: Bool <- memIfc.(mem_readTag) memTagAddr;
 
-    Definition getRevokerOffset (a: ty Addr): Expr ty (Bit (Z.log2_up RevokerSize)) :=
-      TruncMsb (Z.log2_up RevokerSize) (Z.log2_up XlenBytes)
-        (TruncLsb (AddrSz - LgRevokerSzBytes) LgRevokerSzBytes (Sub #a RevokerEpochAddr)).
+        Let ldBase: Bit (AddrSz + 1) <- #ldECap`"base";
+        LetA revBit: Bool <- memIfc.(mem_readRevBit) ldBase;
 
-    Definition readRevoker (offset: ty (Bit (Z.log2_up RevokerSize))) (revokerState: ty SpecRevokerAccessState):
-      Expr ty Data :=
-      (Or [ITE0 (Eq #offset $0) ##revokerState`"revokerEpoch";
-           ITE0 (Eq #offset $1) (Const ty Data (bits.of_Z _ 0));
-           ITE0 (Eq #offset $2) (castBits (Zplus_minus _ _)
-                                   (ZeroExtendTo AddrSz ##revokerState`"revokerStart"));
-           ITE0 (Eq #offset $3) (castBits (Zplus_minus _ _)
-                                   (ZeroExtendTo AddrSz ##revokerState`"revokerEnd"))]).
+        Let ldTagFinal: Bool <- ITE #isCap (And [#ldTag; Not #revBit]) ConstDef;
+        Return ((STRUCT { "tag" ::= #ldTagFinal;
+                          "ecap" ::= #ldECapFinal;
+                          "addr" ::= #ldVal }) : Expr ty FullECapWithTag) ).
 
-    Definition getRevokerAddr (a: ty Addr): Expr ty (Bit MemWidthCap).
-      refine
-        (TruncMsb MemWidthCap LgNumBytesFullCapSz
-           (castBits _ (TruncLsb (AddrSz - Z.of_nat MemWidth) (Z.of_nat MemWidth) (castBits _ #a)))).
-      - abstract (unfold MemWidthCap; lia).
-      - abstract (unfold AddrSz; lia).
-    Defined.
-
-    Definition writeRevoker (offset: ty (Bit (Z.log2_up RevokerSize))) (d: ty Data) (old: ty SpecRevokerAccessState)
-      : Expr ty SpecRevokerAccessState :=
-      STRUCT {
-          "revokerEpoch" ::= ITE (Eq #offset $0) #d ##old`"revokerEpoch";
-          "revokerKick" ::= Eq #offset $1;
-          "revokerStart" ::= ITE (Eq #offset $2) (getRevokerAddr d) #old`"revokerStart";
-          "revokerEnd" ::= ITE (Eq #offset $3) (getRevokerAddr d) #old`"revokerEnd"
-        }.
-
-  #[projections(primitive)]
-  Record MemIfc {ty: Kind -> Type} := {
-    mem_readBytes: ty Addr -> ty (Bit MemSz) -> Expr ty (Array (Z.to_nat DXlenBytes) (Bit 8));
-    mem_readTag: forall {m}, ty (Bit m) -> Expr ty Bool;
-    mem_readRevBit: ty (Bit (AddrSz + 1)) -> Expr ty Bool;
-    mem_writeBytes: ty Addr -> ty (Array (Z.to_nat DXlenBytes) (Bit 8)) -> ty (Bit MemSz) -> Action ty mem_t (Bit 0);
-    mem_writeTag: forall {m}, ty (Bit m) -> ty Bool -> Action ty mem_t (Bit 0)
-  }.
-
-    Definition interrupts: Action ty specTree (Bit 0) :=
-      ( Get interrupts <- ".interrupts_in" in specTree;
-        RegRead specInterrupts <- ".interrupts" in specTree;
-        RegWrite ".interrupts" in specTree <- Or [#interrupts; #specInterrupts];
-        Retv ).
-
-    Variable memIfc: MemIfc (ty:=ty).
-
-    Definition np_mem: NodePath specTree mem_t := ltac:(solveNodePath specTree ".mem"%string mem_t).
-
-    Ltac specSimpl x :=
-      let x' := eval cbv [decode alu encodeCap decodeCap readRevoker writeRevoker getRevokerAddr
-                           revokerKickInit revokerEpochInit revokerStartInit revokerEndInit] in x in
-      let x'' := eval cbn in x' in
-      exact x''.
-    Notation specSimpl x := ltac:(specSimpl x) (only parsing).
+    Definition memStore (memAddr: ty Addr) (memSz: ty (Bit MemSzSz))
+                        (stTag: ty Bool) (stECap: ty ECap) (stVal: ty Addr)
+                        (Store: ty Bool)
+      : Action ty mem_t (Bit 0) :=
+      ( Let isCap : Bool <- isAllOnes #memSz;
+        LetL stCap: Cap <- encodeCap stECap;
+        Let stBits: Bit DXlen <- {< ToBit #stCap, #stVal >};
+        Let memTagAddr: Bit (AddrSz - MemSz) <- TruncMsb _ MemSz #memAddr;
+        
+        If #Store
+        Then (
+          Act memIfc.(mem_writeBits) memAddr stBits memSz;
+          If #isCap
+          Then (Act memIfc.(mem_writeTag) memTagAddr stTag; Retv);
+          If (Eq #memAddr (Const ty _ tohostAddr))
+          Then (
+            If (Eq #stVal $1)
+            Then (
+              System [DispString ty "SUCCESS"%string] Retv )
+            Else (
+              System [DispString ty "FAILURE"%string] Retv );
+            Retv );
+          Retv );
+        Retv).
 
     Definition cpuAction: Action ty specTree (Bit 0) :=
       ( RegRead regs <- ".regs" in specTree;
         RegRead csrs <- ".csrs" in specTree;
         RegRead scrs <- ".scrs" in specTree;
         RegRead interrupts <- ".interrupts" in specTree;
-        RegRead revokerEpoch <- ".revokerEpoch" in specTree;
-        RegRead revokerKick <- ".revokerKick" in specTree;
-        RegRead revokerStart <- ".revokerStart" in specTree;
-        RegRead revokerEnd <- ".revokerEnd" in specTree;
-        RegRead revokeAddr <- ".revokeAddr" in specTree;
 
-        Let revoker : SpecRevokerAccessState <- STRUCT { "revokerEpoch" ::= #revokerEpoch;
-                                                         "revokerKick" ::= #revokerKick;
-                                                         "revokerStart" ::= #revokerStart;
-                                                         "revokerEnd" ::= #revokerEnd };
-
-        Let insts : Array binaryLength (Bit 8) <- Const ty _ specInst;
         Let pcc : FullECapWithTag <- #regs $[ 0 ];
         Let pcVal : Addr <- #pcc`"addr";
-        Let BoundsException : Bool <- And [Slt (ZeroExtend 1 #pcVal) (##pcc`"ecap"`"top"); Sge (ZeroExtend 1 #pcVal) (##pcc`"ecap"`"base")];
+        Let BoundsException : Bool <- And [ Sge (ZeroExtend 1 #pcVal) (##pcc`"ecap"`"base");
+                                            Slt (ZeroExtend 1 #pcVal) (##pcc`"ecap"`"top")];
         Let pcAluOut: PcAluOut <- STRUCT { "pcVal" ::= #pcVal;
                                            "BoundsException" ::= #BoundsException };
-        Let inst: Inst <- ToBit (slice #insts #pcVal (Z.to_nat InstSz/8));
+        LetA inst: Inst <- liftAction np_mem (memIfc.(mem_readInst) pcVal);
         LetL decodeOut: DecodeOut <- decode inst;
 
         Let aluIn: AluIn <- STRUCT { "pcAluOut" ::= #pcAluOut;
-                                      "decodeOut" ::= #decodeOut;
-                                      "regs" ::= #regs;
-                                      "waits" ::= Const ty (Array NumRegs Bool) (Default _);
-                                      "csrs" ::= #csrs;
-                                      "scrs" ::= #scrs;
-                                      "interrupts" ::= #interrupts };
+                                     "decodeOut" ::= #decodeOut;
+                                     "regs" ::= #regs;
+                                     "waits" ::= Const ty (Array NumRegs Bool) (Default _);
+                                     "csrs" ::= #csrs;
+                                     "scrs" ::= #scrs;
+                                     "interrupts" ::= #interrupts };
         Let pcTag <- #pcc`"tag";
         Let pcCap <- #pcc`"ecap";
         LetL aluOut: AluOut <- alu pcTag pcCap aluIn;
         Let memAddr: Addr <- ##aluOut`"multicycleOp"`"memAddr";
-        Let memSz: Bit MemSz <- Sll $1 (##aluOut`"multicycleOp"`"memSz");
-        Let isCap: Bool <- isZero #memSz;
+        Let memSz: Bit MemSzSz <- ##aluOut`"multicycleOp"`"memSz";
         Let ldUn: Bool <- ##aluOut`"multicycleOp"`"LoadUnsigned";
-
-        Let isRevoker: Bool <- isRevokerAddr memAddr memSz;
-        Let revokerOffset: Bit (Z.log2_up RevokerSize) <- getRevokerOffset memAddr;
-        Let revokerData: Data <- readRevoker revokerOffset revoker;
-
-        Let bytes: Array (Z.to_nat DXlenBytes) (Bit 8) <- memIfc.(mem_readBytes) memAddr memSz;
-        Let fullCap: FullCap <- FromBit FullCap (ToBit (k := Array _ _) #bytes);
-        Let ldCap: Cap <- #fullCap`"cap";
-        Let ldVal: Array (Z.to_nat XlenBytes) (Bit 8) <- FromBit (Array (Z.to_nat XlenBytes) (Bit 8))
-                                                           (ITE #isRevoker #revokerData #fullCap`"addr");
-        Let ldValFinal <- ToBit (ITE #ldUn (ArrayZeroExtend #memSz #ldVal) (ArraySignExtend #memSz #ldVal));
-        LetL ldECap: ECap <- decodeCap ldCap ldValFinal;
-        Let ldECapFinal: ECap <- ITE #isCap #ldECap ConstDef;
         Let memTagAddr: Bit (AddrSz - MemSz) <- TruncMsb _ MemSz #memAddr;
 
-        Let ldTag: Bool <- memIfc.(mem_readTag) memTagAddr;
-
-        Let ldBase: Bit (AddrSz + 1) <- #ldECap`"base";
-        Let revBit: Bool <- memIfc.(mem_readRevBit) ldBase;
-
-        Let ldTagFinal: Bool <- ITE #isCap (And [#ldTag; Not #revBit]) ConstDef;
-        Let ldFinal: FullECapWithTag <- STRUCT { "tag" ::= #ldTagFinal;
-                                                 "ecap" ::= #ldECapFinal;
-                                                 "addr" ::= #ldValFinal };
+        LetA ldFinal: FullECapWithTag <- liftAction np_mem (memLoad memAddr memSz ldUn);
 
         Let ldRegIdx <- ##aluOut`"multicycleOp"`"loadRegIdx";
-        Let aluOutRegs: Array NumRegs FullECapWithTag <- eq_rect _ (fun k => Expr ty k) (##aluOut`"regs") _ eq_refl;
+        Let aluOutRegs: Array NumRegs FullECapWithTag <- ##aluOut`"regs";
         Let newRegs: Array NumRegs FullECapWithTag <- #aluOutRegs
                                                           @[ #ldRegIdx <- ITE (##aluOut`"multicycleOp"`"Load")
                                                                             #ldFinal
@@ -248,93 +180,31 @@ Section Spec.
         Let stECap: ECap <- ##aluOut`"multicycleOp"`"storeVal"`"ecap";
 
         Let stVal <- ##aluOut`"multicycleOp"`"storeVal"`"addr";
-        LetL stCap: Cap <- encodeCap stECap;
-        Let stBits: Bit DXlen <- {< ToBit #stCap, #stVal >};
-        Let stBytes: Array (Z.to_nat DXlenBytes) (Bit 8) <- FromBit (Array (Z.to_nat DXlenBytes) (Bit 8)) #stBits;
         Let Store: Bool <- ##aluOut`"multicycleOp"`"Store";
-        Let StoreMem: Bool <- And [#Store; Not #isRevoker];
-        Let newRevoker <- ITE (And [#Store; #isRevoker])
-                                  (writeRevoker revokerOffset stVal revoker)
-                                  #revoker;
-
         Let stTag: Bool <- ##aluOut`"multicycleOp"`"storeVal"`"tag";
-        LetIf _ <- If #StoreMem
-        Then (
-          Act liftAction np_mem (memIfc.(mem_writeBytes) memAddr stBytes memSz);
-          If #isCap
-            Then (Act liftAction np_mem (memIfc.(mem_writeTag) memTagAddr stTag); Retv)
-            Else Retv;
-          Retv
-        ) Else (Retv);
 
-        LetIf _ <- If And [#StoreMem; Eq #memAddr (Const ty _ tohostAddr)]
-        Then (
-          LetIf _ <- If (Eq #stVal $1)
-          Then (
-            System [DispString ty "SUCCESS"%string] Retv )
-          Else (
-            System [DispString ty "FAILURE"%string] Retv );
-          Retv )
-        Else (Retv);
+        Act liftAction np_mem (memStore memAddr memSz stTag stECap stVal Store);
 
         RegWrite ".regs" in specTree <- #newRegs;
         RegWrite ".csrs" in specTree <- #aluOut`"csrs";
         RegWrite ".scrs" in specTree <- ##aluOut`"scrs";
         RegWrite ".interrupts" in specTree <- ##aluOut`"interrupts";
-        RegWrite ".revokerEpoch" in specTree <- ##newRevoker`"revokerEpoch";
-        RegWrite ".revokerKick" in specTree <- ##newRevoker`"revokerKick";
-        RegWrite ".revokerStart" in specTree <- ##newRevoker`"revokerStart";
-        RegWrite ".revokerEnd" in specTree <- ##newRevoker`"revokerEnd";
         Retv ).
 
-    Lemma revoker_addr_size_eq : (0 + MemSz + MemWidthCap + (32 - (0 + MemSz + MemWidthCap)) = 32)%Z.
-    Proof.
-      lia.
-    Qed.
-
-    Definition revoker: Action ty specTree (Bit 0) :=
-      ( RegRead revokerEpoch <- ".revokerEpoch" in specTree;
-        RegRead revokerKick <- ".revokerKick" in specTree;
-        RegRead revokerStart <- ".revokerStart" in specTree;
-        RegRead revokerEnd <- ".revokerEnd" in specTree;
-        RegRead revokeAddr <- ".revokeAddr" in specTree;
-
-        Let ldTag: Bool <- memIfc.(mem_readTag) revokeAddr;
-        Let rvkAddr : Addr <- @castBits ty _ 32 revoker_addr_size_eq (ZeroExtendTo 32 {< #revokeAddr, Const ty (Bit MemSz) (bits.of_Z _ 0) >});
-        Let rvkSz : Bit MemSz <- Const ty (Bit MemSz) (bits.of_Z _ 0);
-        Let bytes: Array (Z.to_nat DXlenBytes) (Bit 8) <- memIfc.(mem_readBytes) rvkAddr rvkSz;
-        Let fullCap: FullCap <- FromBit FullCap (ToBit (k := Array _ _) #bytes);
-        Let ldCap: Cap <- #fullCap`"cap";
-        Let ldVal: Addr <- #fullCap`"addr";
-        LetL ldECap: ECap <- decodeCap ldCap ldVal;
-        Let ldBase <- #ldECap`"base";
-        Let revBit: Bool <- memIfc.(mem_readRevBit) ldBase;
-        Let ldTagFinal <- And [#ldTag; Not #revBit];
-        Act liftAction np_mem (memIfc.(mem_writeTag) revokeAddr ldTagFinal);
-
-        Let workStart <- And [Eq #revokeAddr #revokerEnd; #revokerKick];
-        Let doWork <- Slt #revokeAddr #revokerEnd;
-        Let incRevokeAddr <- Add [#revokeAddr; $1];
-        Let newRevokeAddr <- ITE #workStart
-                                #revokerStart
-                                (ITE #doWork
-                                   #incRevokeAddr
-                                   #revokeAddr);
-        Let newEpoch <- Add [#revokerEpoch; ITE (Or [Eq #incRevokeAddr #revokerEnd; #workStart]) $1 $0];
-
-        RegWrite ".revokerEpoch" in specTree <- #newEpoch;
-        RegWrite ".revokerKick" in specTree <- Const ty Bool false;
-        RegWrite ".revokeAddr" in specTree <- #newRevokeAddr;
+      Definition interrupts: Action ty specTree (Bit 0) :=
+      ( Get interrupts <- ".interrupts_in" in specTree;
+        RegRead currInterrupts <- ".interrupts" in specTree;
+        RegWrite ".interrupts" in specTree <- Or [#interrupts; #currInterrupts];
         Retv ).
   End Ty.
 
-  Definition spec (memIfc : forall ty, MemIfc (ty:=ty)) : Mod specTree :=
-    fun ty => [cpuAction (memIfc ty); interrupts ty; revoker (memIfc ty)].
+  Definition spec (memIfc : forall ty, @MemIfc mem_t ty) : Mod specTree :=
+    fun ty => [cpuAction (memIfc ty); interrupts ty].
 
   Definition SpecInvariant (s: TreeState ElemState specTree) : Prop.
   Admitted.
 
-  Theorem specInvariantPreserved: forall (memIfc : MemIfc (ty:=type)) old new,
+  Theorem specInvariantPreserved: forall (memIfc : @MemIfc mem_t type) old new,
       SpecInvariant old ->
       SemAction (cpuAction memIfc) old new Zmod.zero ->
       SpecInvariant new.
@@ -346,23 +216,12 @@ Section Spec.
       SpecInvariant new.
   Admitted.
 
-  Theorem revokerInvariantPreserved: forall (memIfc : MemIfc (ty:=type)) old new,
-      SpecInvariant old ->
-      SemAction (revoker memIfc) old new Zmod.zero ->
-      SpecInvariant new.
-  Admitted.
-
   Ltac simplifyAluExpr v :=
     let x := eval cbn delta -[evalFromBitStruct] beta iota in v in
       let x := eval cbv delta [mapSameTuple updSameTuple updSameTupleNat Bool.transparent_Is_true]
                  beta iota in x in
         let x := eval cbn delta -[evalFromBitStruct] beta iota in x in
           x.
-
-  (*
-  Definition evalCpuActionExpr (state: Expr type AllSpecState): type AllSpecState :=
-    ltac:(let x := simplifyAluExpr (evalLetExpr (cpuActionExpr state)) in exact x).
-  *)
 End Spec.
 
 Section PartialInitSpec.
@@ -370,7 +229,7 @@ Section PartialInitSpec.
   Local Open Scope guru_scope.
 
   Variable MemWidth: nat.
-  Variable MemWidthGeLgBytesFullCapSz: MemWidth >= LgBytesFullCapSz.
+  Variable MemWidthGeLgBytesFullCapSz: MemWidth >= Z.to_nat LgNumBytesFullCapSz.
   Variable regsInit: type (Array NumRegs FullECapWithTag).
 
   Variable regsInitPc:
@@ -383,6 +242,160 @@ Section PartialInitSpec.
                                         "mepcc" ::= ExecRoot }.
 
   Variable mem_t: Tree Elem.
-  Definition partialInitSpec (memIfc : forall ty, MemIfc mem_t (ty:=ty)) := spec (mem_t:=mem_t) MemWidthGeLgBytesFullCapSz (Default _) regsInit scrsInit
-                                                                              (Default _) (Default _) (Default _) (Default _) (Default _) (Default _) (Default _) 0%Z memIfc.
+  Definition partialInitSpec (memIfc : forall ty, @MemIfc mem_t ty) :=
+    spec (mem_t:=mem_t) (Default _) regsInit scrsInit
+         (Default _) (Default _) memIfc.
 End PartialInitSpec.
+
+Section Uncore.
+  Variable RevokerStartAddrAligned: Z.
+  Definition RevokerNumRegs : Z := 4.
+  Definition RevokerSizeBytes : Z := XlenBytes * RevokerNumRegs.
+  Definition RevokerAlignBits : Z := Z.log2_up RevokerSizeBytes.
+
+  Variable revokerEpochInit: type Data.
+  Variable revokerKickInit: type Bool.
+  Variable revokerStartInit: type (Bit (AddrSz - LgNumBytesFullCapSz)).
+  Variable revokerEndInit: type (Bit (AddrSz - LgNumBytesFullCapSz)).
+  Variable revokeAddrInit: type (Bit (AddrSz - LgNumBytesFullCapSz)).
+
+  Local Open Scope string_scope.
+  Local Open Scope guru_scope.
+
+  Variable mem_t: Tree Elem.
+
+  Definition uncoreTree : Tree Elem :=
+    Node "" [
+      Node "mem" [mem_t];
+      Node "revoker" [
+        Leaf "revokerEpoch" (EReg {| regKind := Data; regInit := Some revokerEpochInit |});
+        Leaf "revokerKick" (EReg {| regKind := Bool; regInit := Some revokerKickInit |});
+        Leaf "revokerStart" (EReg {| regKind := Bit (AddrSz - LgNumBytesFullCapSz); regInit := Some revokerStartInit |});
+        Leaf "revokerEnd" (EReg {| regKind := Bit (AddrSz - LgNumBytesFullCapSz); regInit := Some revokerEndInit |});
+        Leaf "revokeAddr" (EReg {| regKind := Bit (AddrSz - LgNumBytesFullCapSz); regInit := Some revokeAddrInit |})
+      ]
+    ].
+
+  Definition uncore_np_mem: NodePath uncoreTree mem_t := ltac:(solveNodePath uncoreTree ".mem"%string mem_t).
+
+  Definition RevokerStartAddr : Z :=
+    Z.shiftl RevokerStartAddrAligned RevokerAlignBits.
+
+  Definition RevokerEndAddr : Z :=
+    Z.lor RevokerStartAddr (RevokerSizeBytes-1).
+
+  Section Ty.
+    Variable ty: Kind -> Type.
+    Variable rawMemIfc: @MemIfc mem_t ty.
+
+    Definition isRevokerAddr (a: Expr ty Addr) :=
+      And [Sge a $RevokerStartAddr; Sle a $RevokerEndAddr].
+
+    Definition getRevokerOffset (a: ty Addr): Expr ty (Bit 2) :=
+      TruncMsb (Z.log2_up RevokerNumRegs) (Z.log2_up XlenBytes)
+        (TruncLsb (AddrSz - RevokerAlignBits) RevokerAlignBits #a).
+
+    Definition uncoreMemIfc : @MemIfc uncoreTree ty := {|
+      mem_readBits := fun addr =>
+        ( Let isRevoker: Bool <- isRevokerAddr #addr;
+          Let offset: Bit 2 <- getRevokerOffset addr;
+          LetIf retVal : Bit DXlen <- If #isRevoker
+          Then (
+            RegRead revokerEpoch <- ".revoker.revokerEpoch" in uncoreTree;
+            RegRead revokerStart <- ".revoker.revokerStart" in uncoreTree;
+            RegRead revokerEnd <- ".revoker.revokerEnd" in uncoreTree;
+            Let revokerVal: Data <-
+              (Or [ITE0 (Eq #offset $0) ##revokerEpoch;
+                   ITE0 (Eq #offset $1) (Const ty Data (bits.of_Z _ 0));
+                   ITE0 (Eq #offset $2) {< ##revokerStart, Const ty (Bit LgNumBytesFullCapSz) Zmod.zero >};
+                   ITE0 (Eq #offset $3) {< ##revokerEnd, Const ty (Bit LgNumBytesFullCapSz) Zmod.zero >}]);
+            Return (ZeroExtendTo DXlen #revokerVal)
+          ) Else (liftAction uncore_np_mem (rawMemIfc.(mem_readBits) addr));
+          Return #retVal );
+      mem_readTag := fun addr =>
+        liftAction uncore_np_mem (rawMemIfc.(mem_readTag) addr);
+      mem_readRevBit := fun addr =>
+        liftAction uncore_np_mem (rawMemIfc.(mem_readRevBit) addr);
+      mem_readInst := fun addr =>
+        liftAction uncore_np_mem (rawMemIfc.(mem_readInst) addr);
+      mem_writeBits := fun addr val sz =>
+        ( Let isRevoker: Bool <- isRevokerAddr #addr;
+          Let offset: Bit 2 <- getRevokerOffset addr;
+          Let alignedAddr <- TruncMsb (AddrSz - LgNumBytesFullCapSz) LgNumBytesFullCapSz #addr;
+          If #isRevoker
+          Then (
+            (* TODO: update only upto sz bytes; keep the rest of the value same as what we had earlier *)
+            If (Eq #offset $0)
+            Then (
+              RegRead oldEpoch <- ".revoker.revokerEpoch" in uncoreTree;
+              Let newEpoch : Data <- TruncLsb Xlen Xlen #val;
+              Let updatedEpoch : Data <- updateWordByByteSz #sz #oldEpoch #newEpoch;
+              RegWrite ".revoker.revokerEpoch" in uncoreTree <- #updatedEpoch;
+              Retv
+            );
+            If (Eq #offset $1)
+            Then (
+              RegWrite ".revoker.revokerKick" in uncoreTree <- (Const ty Bool true);
+              Retv
+            );
+            If (Eq #offset $2)
+            Then (
+              RegRead oldStart <- ".revoker.revokerStart" in uncoreTree;
+              Let oldAddr : Addr <- {< #oldStart, Const ty (Bit LgNumBytesFullCapSz) Zmod.zero >};
+              Let newAddr : Addr <- TruncLsb Xlen Xlen #val;
+              Let updatedAddr : Addr <- updateWordByByteSz #sz #oldAddr #newAddr;
+              RegWrite ".revoker.revokerStart" in uncoreTree <- TruncMsb (AddrSz - LgNumBytesFullCapSz) LgNumBytesFullCapSz #updatedAddr;
+              Retv
+            );
+            If (Eq #offset $3)
+            Then (
+              RegRead oldEnd <- ".revoker.revokerEnd" in uncoreTree;
+              Let oldAddr : Addr <- {< #oldEnd, Const ty (Bit LgNumBytesFullCapSz) Zmod.zero >};
+              Let newAddr : Addr <- TruncLsb Xlen Xlen #val;
+              Let updatedAddr : Addr <- updateWordByByteSz #sz #oldAddr #newAddr;
+              RegWrite ".revoker.revokerEnd" in uncoreTree <- TruncMsb (AddrSz - LgNumBytesFullCapSz) LgNumBytesFullCapSz #updatedAddr;
+              Retv
+            );
+            Retv
+          ) Else (liftAction uncore_np_mem (rawMemIfc.(mem_writeBits) addr val sz));
+          Retv );
+      mem_writeTag := fun addr tag =>
+        liftAction uncore_np_mem (rawMemIfc.(mem_writeTag) addr tag)
+    |}.
+
+    (* TODO: Check with Wes about this design *)
+    Definition revoker: Action ty uncoreTree (Bit 0) :=
+      ( RegRead revokerEpoch <- ".revoker.revokerEpoch" in uncoreTree;
+        RegRead revokerKick <- ".revoker.revokerKick" in uncoreTree;
+        RegRead revokerStart <- ".revoker.revokerStart" in uncoreTree;
+        RegRead revokerEnd <- ".revoker.revokerEnd" in uncoreTree;
+        RegRead revokeAddr <- ".revoker.revokeAddr" in uncoreTree;
+
+        Let waiting <- Sge #revokeAddr #revokerEnd;
+
+        If (Not #waiting)
+        Then (
+          Let revokeAddrFull : Addr <- {< #revokeAddr, ConstDefK (Bit LgNumBytesFullCapSz) >};
+          LetA ldTag: Bool <- liftAction uncore_np_mem (rawMemIfc.(mem_readTag) revokeAddr);
+          LetA bits: Bit DXlen <- liftAction uncore_np_mem (rawMemIfc.(mem_readBits) revokeAddrFull);
+          Let fullCap: FullCap <- FromBit FullCap #bits;
+          Let ldCap: Cap <- #fullCap`"cap";
+          Let ldVal: Addr <- #fullCap`"addr";
+          LetL ldECap: ECap <- decodeCap ldCap ldVal;
+          Let ldBase <- #ldECap`"base";
+          LetA revBit: Bool <- liftAction uncore_np_mem (rawMemIfc.(mem_readRevBit) ldBase);
+          Let ldTagFinal <- And [#ldTag; Not #revBit];
+          Act (liftAction uncore_np_mem (rawMemIfc.(mem_writeTag) revokeAddr ldTagFinal));
+          RegWrite ".revoker.revokeAddr" in uncoreTree <- Add [#revokeAddr; $1];
+          Retv)
+        Else (
+          If (#revokerKick)
+            Then (
+              RegWrite ".revoker.revokerEpoch" in uncoreTree <- Add [#revokerEpoch; $1];
+              RegWrite ".revoker.revokerKick" in uncoreTree <- ConstDef;
+              RegWrite ".revoker.revokeAddr" in uncoreTree <- #revokerStart;
+              Retv );
+          Retv);
+        Retv ).
+  End Ty.
+End Uncore.
